Some lemmas and fixes

compiler/backend/pure_cexpScript.sml
@@ -131,4 +131,39 @@ Definition get_info_def:
   get_info (Case c _ _ _) = c
 End
 
+Definition cexp_wf_def:
+  cexp_wf (Var _ v) = T ∧
+  cexp_wf (Prim _ op es) = EVERY cexp_wf es ∧
+  cexp_wf (App _ e es) = (cexp_wf e ∧ EVERY cexp_wf es ∧ es ≠ []) ∧
+  cexp_wf (Lam _ vs e) = (cexp_wf e ∧ vs ≠ []) ∧
+  cexp_wf (Let _ v e1 e2) = (cexp_wf e1 ∧ cexp_wf e2) ∧
+  cexp_wf (Letrec _ fns e) = (EVERY cexp_wf $ MAP SND fns ∧ cexp_wf e ∧ fns ≠ []) ∧
+  cexp_wf (Case _ e v css) = (
+    cexp_wf e ∧ EVERY cexp_wf $ MAP (SND o SND) css ∧ css ≠ [])
+Termination
+  WF_REL_TAC `measure $ cexp_size (K 0)` >> rw[fetch "-" "cexp_size_def"] >>
+  gvs[MEM_MAP, EXISTS_PROD] >>
+  rename1 `MEM _ es` >> Induct_on `es` >> rw[] >> gvs[fetch "-" "cexp_size_def"]
+End
+
+Definition cexp_eq_def:
+  cexp_eq (Var _ v1) (Var _ v2) = (v1 = v2) ∧
+  cexp_eq (Prim _ op1 es1) (Prim _ op2 es2) = (
+    op1 = op2 ∧ LIST_REL (λe1 e2. cexp_eq e1 e2) es1 es2) ∧
+  cexp_eq (App _ e1 es1) (App _ e2 es2) = (
+    cexp_eq e1 e2 ∧ LIST_REL (λe1 e2. cexp_eq e1 e2) es1 es2) ∧
+  cexp_eq (Lam _ vs1 e1) (Lam _ vs2 e2) = (vs1 = vs2 ∧ cexp_eq e1 e2) ∧
+  cexp_eq (Let _ v1 e11 e12) (Let _ v2 e21 e22) = (
+    v1 = v2 ∧ cexp_eq e11 e21 ∧ cexp_eq e12 e22) ∧
+  cexp_eq (Letrec _ fns1 e1) (Letrec _ fns2 e2) = (cexp_eq e1 e2 ∧
+    LIST_REL (λ(fn1,e1) (fn2,e2). fn1 = fn2 ∧ cexp_eq e1 e2) fns1 fns2) ∧
+  cexp_eq (Case _ e1 v1 css1) (Case _ e2 v2 css2) = (
+    cexp_eq e1 e2 ∧ v1 = v2 ∧
+    LIST_REL (λ(cn1,vs1,e1) (cn2,vs2,e2). cn1 = cn2 ∧ vs1 = vs2 ∧ cexp_eq e1 e2)
+      css1 css2)
+Termination
+  WF_REL_TAC `measure $ cexp_size (K 0) o SND` >> rw[fetch "-" "cexp_size_def"] >>
+  rename1 `MEM _ es` >> Induct_on `es` >> rw[] >> gvs[fetch "-" "cexp_size_def"]
+End
+
 val _ = export_theory();
