typing/pure_typingPropsScript.sml
@@ -1,7 +1,7 @@
 open HolKernel Parse boolLib bossLib BasicProvers;
 open pairTheory arithmeticTheory integerTheory stringTheory optionTheory
      listTheory alistTheory;
-open pure_cexpTheory pure_configTheory pure_typingTheory
+open pure_miscTheory pure_cexpTheory pure_configTheory pure_typingTheory
 
 val _ = new_theory "pure_typingProps";
 
@@ -9,11 +9,53 @@ val _ = new_theory "pure_typingProps";
 (******************** Substitutions and shifts ********************)
 
 Theorem shift_db_0[simp]:
-  shift_db skip 0 t = t
+  ∀t skip. shift_db skip 0 t = t
 Proof
   qsuff_tac `∀skip n t. n = 0 ⇒ shift_db skip n t = t` >- gvs[] >>
   recInduct shift_db_ind >> rw[shift_db_def] >>
   rw[LIST_EQ_REWRITE] >> gvs[MEM_EL, PULL_EXISTS, EL_MAP]
+QED
+
+Theorem subst_db_unchanged:
+  ∀skip ts t n.
+    freetyvars_ok n t ∧
+    n ≤ skip
+  ⇒ subst_db skip ts t = t
+Proof
+  recInduct subst_db_ind >> reverse $ rw[subst_db_def, freetyvars_ok_def]
+  >- metis_tac[] >>
+  irule MAP_ID_ON >> gvs[EVERY_MEM] >> metis_tac[]
+QED
+
+Theorem shift_db_unchanged:
+  ∀skip shift t n.
+    freetyvars_ok n t ∧
+    n ≤ skip
+  ⇒ shift_db skip shift t = t
+Proof
+  recInduct shift_db_ind >> reverse $ rw[shift_db_def, freetyvars_ok_def]
+  >- metis_tac[] >>
+  irule MAP_ID_ON >> gvs[EVERY_MEM] >> metis_tac[]
+QED
+
+Theorem subst_db_shift_db:
+  ∀skip shift t ts m.
+    (m - skip) + LENGTH ts ≤ shift ∧
+    skip ≤ m
+  ⇒ subst_db m ts (shift_db skip shift t) =
+    shift_db skip (shift - LENGTH ts) t
+Proof
+  recInduct shift_db_ind >> rw[subst_db_def, shift_db_def] >>
+  rw[MAP_MAP_o, combinTheory.o_DEF, MAP_EQ_f]
+QED
+
+Theorem tsubst_tshift:
+  ∀shift t ts m.
+    LENGTH ts ≤ shift
+  ⇒ tsubst ts (tshift shift t) =
+    tshift (shift - LENGTH ts) t
+Proof
+  rw[] >> irule subst_db_shift_db >> simp[]
 QED
 
 
@@ -79,6 +121,37 @@ Proof
   gvs[EVERY_MAP, EVERY_MEM]
 QED
 
+Theorem type_ok_mono:
+  ∀tdefs n m t.
+    type_ok tdefs n t ∧
+    n ≤ m
+  ⇒ type_ok tdefs m t
+Proof
+  rw[type_ok_def] >> drule_all freetyvars_ok_mono >> simp[]
+QED
+
+Theorem type_ok_subst_db:
+  ∀skip ts tdefs n.
+    type_ok tdefs (n + LENGTH ts) t ∧
+    EVERY (type_ok tdefs n) ts ∧
+    skip ≤ n
+  ⇒ type_ok tdefs n (subst_db skip ts t)
+Proof
+  rw[type_ok_def]
+  >- (irule freetyvars_ok_subst_db >> gvs[EVERY_MEM, type_ok_def])
+  >- (irule type_wf_subst_db >> gvs[EVERY_MEM, type_ok_def])
+QED
+
+Theorem type_ok_shift_db:
+  ∀skip shift tdefs n t.
+    type_ok tdefs n t
+  ⇒ type_ok tdefs (n + shift) (shift_db skip shift t)
+Proof
+  rw[type_ok_def]
+  >- (irule freetyvars_ok_shift_db >> gvs[EVERY_MEM, type_ok_def])
+  >- (irule type_wf_shift_db >> gvs[EVERY_MEM, type_ok_def])
+QED
+
 Theorem type_ok:
   (∀tds v n. type_ok tds n (TypeVar v) ⇔ v < n) ∧
   (∀tds p n. type_ok tds n (PrimTy p) ⇔ T) ∧
@@ -135,7 +208,7 @@ Proof
       disch_then $ qspecl_then [`b`,`new`] assume_tac >> gvs[]
       )
     >- (
-      drule freetyvars_ok_mono >> disch_then irule >> simp[]
+      irule freetyvars_ok_shift_db >> first_x_assum irule >> simp[]
       )
     )
   >- (
@@ -166,39 +239,31 @@ Proof
   gvs[LIST_REL_EL_EQN, IMP_CONJ_THM, FORALL_AND_THM]
   >- (
     PairCases_on `s` >> gvs[specialises_def] >>
-    imp_res_tac ALOOKUP_MEM >> gvs[EVERY_MEM, type_ok_def] >>
+    imp_res_tac ALOOKUP_MEM >> gvs[EVERY_MEM] >>
     first_x_assum drule >> strip_tac >> gvs[] >>
-    irule_at Any freetyvars_ok_tsubst >> simp[EVERY_MEM] >>
-    irule_at Any type_wf_subst_db >> simp[EVERY_MEM]
+    irule type_ok_subst_db >> simp[EVERY_MEM]
     )
   >- gvs[EVERY_EL]
-  >- gvs[EVERY_EL, type_ok_def]
+  >- gvs[EVERY_EL]
   >- gvs[type_cons_def]
   >- gvs[oEL_THM, EVERY_EL]
-  >- gvs[EVERY_EL, type_ok_def]
+  >- gvs[EVERY_EL]
   >- (
     first_x_assum irule >>
-    gvs[EVERY_MEM, MEM_ZIP, PULL_EXISTS, EL_MAP, MEM_EL, type_ok_def]
+    gvs[EVERY_MEM, MEM_ZIP, PULL_EXISTS, EL_MAP, MEM_EL]
     )
   >- (
     ntac 2 $ first_x_assum irule >> gvs[EVERY_MEM, FORALL_PROD] >>
-    rw[] >> gvs[MEM_MAP, EXISTS_PROD] >>
+    reverse $ rw[] >> gvs[MEM_MAP, EXISTS_PROD] >>
     first_x_assum drule >> rw[]
-    >- (
-      gvs[type_ok_def] >>
-      drule freetyvars_ok_shift_db >> rename1 `MEM (a,b,c) _` >>
-      disch_then $ qspecl_then [`b`,`new`] assume_tac >> gvs[] >>
-      irule type_wf_shift_db >> simp[]
-      )
-    >- (
-      gvs[type_ok_def] >>
-      drule freetyvars_ok_mono >> disch_then irule >> simp[]
-      )
+    >- (irule type_ok_shift_db >> simp[]) >>
+    rename1 `MEM (a,b,c) _` >>
+    drule type_ok_shift_db >>
+    disch_then $ qspecl_then [`b`,`new`] assume_tac >> gvs[]
     )
   >- (
     first_x_assum irule >>
-    rw[EVERY_EL, EL_ZIP, EL_MAP] >> pairarg_tac >> gvs[EVERY_EL] >>
-    last_x_assum kall_tac >> last_x_assum drule >> simp[]
+    rw[EVERY_EL, EL_ZIP, EL_MAP] >> pairarg_tac >> gvs[EVERY_EL]
     )
   >- (
     gvs[EVERY_MEM, oEL_THM, namespace_ok_def] >>
@@ -208,6 +273,124 @@ Proof
     qpat_x_assum `_ ⇒ type_ok typedefs db t` irule >>
     simp[MEM_ZIP, EL_MAP, PULL_EXISTS] >>
     gvs[MEM_EL, PULL_EXISTS]
+    )
+QED
+
+Theorem type_cexp_cexp_wf:
+  ∀ ns db st env e t.
+    EVERY (type_ok (SND ns) db) st ∧
+    EVERY (λ(v,scheme). type_scheme_ok (SND ns) db scheme) env ∧
+    namespace_ok ns ∧
+    type_cexp ns db st env e t
+  ⇒ cexp_wf e
+Proof
+  Induct_on `type_cexp` >> rw[cexp_wf_def, type_wf_def, type_ok] >>
+  gvs[EVERY_EL, LIST_REL_EL_EQN, EL_ZIP, EL_MAP]
+  >- (
+    imp_res_tac type_cexp_type_ok >>
+    gvs[EVERY_EL, LIST_REL_EL_EQN, type_ok, type_wf_def] >>
+    Cases_on `es` >> gvs[]
+    )
+  >- (
+    imp_res_tac type_cexp_type_ok >>
+    gvs[EVERY_EL, LIST_REL_EL_EQN, type_ok, type_wf_def] >>
+    Cases_on `es` >> gvs[]
+    )
+  >- (Cases_on `xs` >> gvs[])
+  >- (
+    first_x_assum irule >> reverse $ rw[]
+    >- (irule type_ok_shift_db >> simp[]) >>
+    qpat_abbrev_tac `a = EL n env` >> PairCases_on `a` >> gvs[] >>
+    first_x_assum drule >> strip_tac >> gvs[] >>
+    drule type_ok_shift_db >> simp[]
+    )
+  >- (
+    first_x_assum irule >>
+    imp_res_tac type_cexp_type_ok >> pop_assum irule >>
+    gvs[EVERY_EL, LIST_REL_EL_EQN, EL_MAP] >> reverse $ rw[]
+    >- (irule type_ok_shift_db >> simp[]) >>
+    qpat_abbrev_tac `a = EL n env` >> PairCases_on `a` >> gvs[] >>
+    first_x_assum drule >> strip_tac >> gvs[] >>
+    drule type_ok_shift_db >> simp[]
+    )
+  >- (
+    rw[] >> last_x_assum drule >>
+    pairarg_tac >> gvs[] >> pairarg_tac >> gvs[] >> strip_tac >>
+    pop_assum irule >> reverse $ rw[]
+    >- (
+      first_x_assum drule >> strip_tac >> gvs[] >>
+      drule type_ok_shift_db >> simp[]
+      ) >>
+    qmatch_goalsub_abbrev_tac `_ (_ m)` >>
+    PairCases_on `m` >> gvs[] >>
+    first_x_assum drule >> strip_tac >> gvs[] >>
+    drule type_ok_shift_db >> simp[]
+    )
+  >- (
+    rw[] >> first_x_assum drule >> pairarg_tac >> gvs[] >> strip_tac >>
+    pop_assum irule >> gvs[EL_ZIP, EL_MAP] >> rw[] >>
+    imp_res_tac type_cexp_type_ok >> gvs[type_ok, EVERY_EL]
+    )
+  >- (
+    gvs[namespace_ok_def, oEL_THM, EVERY_EL] >>
+    first_x_assum drule >> pairarg_tac >> gvs[] >> rw[] >>
+    imp_res_tac sortingTheory.PERM_LENGTH >>
+    Cases_on `css` >> gvs[]
+    )
+QED
+
+Theorem type_cexp_weaken:
+  ∀ns db st env e t db' st' env'.
+    type_cexp ns db st env e t
+  ⇒ type_cexp ns (db + db') (st ++ st') (env ++ env') e t
+Proof
+  ntac 3 gen_tac >>
+  Induct_on `type_cexp` >> rw[] >> rw[Once type_cexp_cases]
+  >- (
+    simp[ALOOKUP_APPEND] >> PairCases_on `s` >> gvs[specialises_def] >>
+    qexists_tac `subs` >> gvs[] >>
+    irule EVERY_MONOTONIC >> rw[] >> goal_assum $ drule_at Any >> rw[] >>
+    drule type_ok_mono >> simp[]
+    )
+  >- gvs[LIST_REL_EL_EQN]
+  >- metis_tac[]
+  >- (drule type_ok_mono >> simp[])
+  >- metis_tac[]
+  >- metis_tac[]
+  >- (disj1_tac >> goal_assum $ drule_at Any >> gvs[LIST_REL_EL_EQN])
+  >- (
+    goal_assum $ drule_at Any >> gvs[LIST_REL_EL_EQN] >>
+    irule EVERY_MONOTONIC >> rw[] >> goal_assum $ drule_at Any >> rw[] >>
+    drule type_ok_mono >> simp[]
+    )
+  >- gvs[oEL_THM, EL_APPEND_EQN]
+  >- (ntac 2 $ goal_assum $ drule_at Any >> gvs[LIST_REL_EL_EQN])
+  >- metis_tac[]
+  >- (disj1_tac >> qexists_tac `ts` >> gvs[LIST_REL_EL_EQN])
+  >- (disj2_tac >> qexists_tac `ts` >> gvs[LIST_REL_EL_EQN])
+  >- (
+    irule EVERY_MONOTONIC >> rw[] >> goal_assum $ drule_at Any >> rw[] >>
+    drule type_ok_mono >> simp[]
+    )
+  >- (qexistsl_tac [`new`,`t`] >> gvs[])
+  >- (
+    qexists_tac `schemes` >> gvs[LIST_REL_EL_EQN] >> rw[]
+    >- (
+      pairarg_tac >> gvs[] >> pairarg_tac >> gvs[] >>
+      last_x_assum drule >> gvs[]
+      )
+    >- (
+      irule EVERY_MONOTONIC >> rw[] >> goal_assum $ drule_at Any >> rw[] >>
+      pairarg_tac >> gvs[] >> drule type_ok_mono >> simp[]
+      )
+    )
+  >- (
+    rpt $ goal_assum $ drule_at Any >> gvs[] >> qexists_tac `typedef` >>
+    irule_at Any EVERY_MONOTONIC >>
+    goal_assum $ drule_at Any >> rw[] >> pairarg_tac >> gvs[] >>
+    goal_assum $ drule_at Any >> gvs[rich_listTheory.APPEND_ASSOC_CONS] >> rw[] >>
+    irule EVERY_MONOTONIC >> rw[] >> goal_assum $ drule_at Any >> rw[] >>
+    drule type_ok_mono >> simp[]
     )
 QED
 
